chore(chap8): try to prove lemma 8.10

ConcreteSemanticsChapter8/ConcreteSemantics8_1_Stack.thy
@@ -234,7 +234,7 @@ value "ccomp (WHILE Less (V ''u'') (N 1) DO (''u'' ::= Plus (V ''u'') (N 1)))"
 subsection "8.4 Preservation of Semantics"
 
 (* Lemma 8.9  *)
-lemma ccomp_correctness: "(c,s) \<Rightarrow> t \<Longrightarrow> ccomp c \<turnstile> (0,s,stk) \<rightarrow>* (size (ccomp c), t, stk)"
+lemma ccomp_bigstep: "(c,s) \<Rightarrow> t \<Longrightarrow> ccomp c \<turnstile> (0,s,stk) \<rightarrow>* (size (ccomp c), t, stk)"
 proof(induction arbitrary: stk rule: big_step_induct)
 case (Skip s)
   then show ?case by (fastforce)
@@ -282,5 +282,136 @@ goal (1 subgoal):
   ultimately  show ?case 
     by (meson \<open>ccomp (WHILE b DO c) \<turnstile> (0, s1, stk) \<rightarrow>* (size (bcomp b False (size (ccomp c) + 1)), s1, stk)\<close> star_trans)
 qed
+
+text\<open>the other direction is difficult to solve.\<close>
+
+text \<open>The possible successor PCs of an instruction at position \<^term>\<open>n\<close>\<close>
+definition isuccs :: "instr \<Rightarrow> int \<Rightarrow> int set" where
+"isuccs i n = (case i of
+  JMP j \<Rightarrow> {n + 1 + j} |
+  JMPLESS j \<Rightarrow> {n + 1 + j, n + 1} |
+  JMPGE j \<Rightarrow> {n + 1 + j, n + 1} |
+  _ \<Rightarrow> {n +1})"
+
+text \<open>The possible successors PCs of an instruction list\<close>
+definition succs :: "instr list \<Rightarrow> int \<Rightarrow> int set" where
+"succs P n = {s. \<exists>i::int. 0 \<le> i \<and> i < size P \<and> s \<in> isuccs (P!!i) (n+i)}" 
+
+text \<open>Possible exit PCs of a program\<close>
+definition exits :: "instr list \<Rightarrow> int set" where
+"exits P = succs P 0 - {0..< size P}"
+
+primrec 
+  exec_n :: "instr list \<Rightarrow> config \<Rightarrow> nat \<Rightarrow> config \<Rightarrow> bool" 
+  ("_/ \<turnstile> (_ \<rightarrow>^_/ _)" [65,0,1000,55] 55)
+where 
+  "P \<turnstile> c \<rightarrow>^0 c' = (c'=c)" |
+  "P \<turnstile> c \<rightarrow>^(Suc n) c'' = (\<exists>c'. (P \<turnstile> c \<rightarrow> c') \<and> P \<turnstile> c' \<rightarrow>^n c'')"
+
+lemma exec_n_exec:
+  "P \<turnstile> c \<rightarrow>^n c' \<Longrightarrow> P \<turnstile> c \<rightarrow>* c'"
+  by (induct n arbitrary: c) (auto intro: star.step)
+
+lemma exec_0 [intro!]: "P \<turnstile> c \<rightarrow>^0 c" by simp
+
+lemma exec_Suc:
+  "\<lbrakk> P \<turnstile> c \<rightarrow> c'; P \<turnstile> c' \<rightarrow>^n c'' \<rbrakk> \<Longrightarrow> P \<turnstile> c \<rightarrow>^(Suc n) c''" 
+  by (fastforce simp del: split_paired_Ex)
+
+lemma exec_exec_n:
+  "P \<turnstile> c \<rightarrow>* c' \<Longrightarrow> \<exists>n. P \<turnstile> c \<rightarrow>^n c'"
+  by (induct rule: star.induct) (auto intro: exec_Suc)
+    
+lemma exec_eq_exec_n:
+  "(P \<turnstile> c \<rightarrow>* c') = (\<exists>n. P \<turnstile> c \<rightarrow>^n c')"
+  by (blast intro: exec_exec_n exec_n_exec)
+
+lemma exec_n_Nil [simp]:
+  "[] \<turnstile> c \<rightarrow>^k c' = (c' = c \<and> k = 0)"
+  by (induct k) (auto simp: exec1_def)
+
+lemma exec1_exec_n [intro!]:
+  "P \<turnstile> c \<rightarrow> c' \<Longrightarrow> P \<turnstile> c \<rightarrow>^1 c'"
+  by (cases c') simp
+
+lemma exec_n_step:
+  "n \<noteq> n' \<Longrightarrow> 
+  P \<turnstile> (n,stk,s) \<rightarrow>^k (n',stk',s') = 
+  (\<exists>c. P \<turnstile> (n,stk,s) \<rightarrow> c \<and> P \<turnstile> c \<rightarrow>^(k - 1) (n',stk',s') \<and> 0 < k)"
+  by (cases k) auto
+
+lemma exec1_end:
+  "size P <= fst c \<Longrightarrow> \<not> P \<turnstile> c \<rightarrow> c'"
+  by (auto simp: exec1_def)
+
+lemma exec_n_end:
+  "size P <= (n::int) \<Longrightarrow> 
+  P \<turnstile> (n,s,stk) \<rightarrow>^k (n',s',stk') = (n' = n \<and> stk'=stk \<and> s'=s \<and> k =0)"
+  by (cases k) (auto simp: exec1_end)
+
+lemmas exec_n_simps = exec_n_step exec_n_end
+
+lemma succs_simps [simp]: 
+  "succs [ADD] n = {n + 1}"
+  "succs [LOADI v] n = {n + 1}"
+  "succs [LOAD x] n = {n + 1}"
+  "succs [STORE x] n = {n + 1}"
+  "succs [JMP i] n = {n + 1 + i}"
+  "succs [JMPGE i] n = {n + 1 + i, n + 1}"
+  "succs [JMPLESS i] n = {n + 1 + i, n + 1}"
+  by (auto simp: succs_def isuccs_def)
+
+lemma succs_empty [iff]: "succs [] n = {}"
+  by (simp add: succs_def)
+
+lemma succs_Cons:
+  "succs (x#xs) n = isuccs x n \<union> succs xs (1+n)" (is "_ = ?x \<union> ?xs")
+proof
+(*
+goal (2 subgoals):
+ 1. succs (x # xs) n \<subseteq> isuccs x n \<union> succs xs (1 + n)
+ 2. isuccs x n \<union> succs xs (1 + n) \<subseteq> succs (x # xs) n
+*)
+  let ?isuccs = "\<lambda>p P n i::int. 0 \<le> i \<and> i < size P \<and> p \<in> isuccs (P!!i) (n+i)"
+  have "p \<in> ?x \<union> ?xs" if assm: "p \<in> succs (x#xs) n" for p
+    sorry
+  thus "succs (x#xs) n \<subseteq> ?x \<union> ?xs" ..
+  have "p \<in> succs (x#xs) n" if assm: "p \<in> ?x \<or> p \<in> ?xs" for p
+    sorry
+  thus "?x \<union> ?xs \<subseteq> succs (x#xs) n" by blast
+qed
+lemma succs_shift:
+  "(p - n \<in> succs P 0) = (p \<in> succs P n)" 
+  by (fastforce simp: succs_def isuccs_def split: instr.split)
+lemma inj_op_plus [simp]:
+  "inj ((+) (i::int))"
+  by (metis add_minus_cancel inj_on_inverseI)
+
+lemma succs_set_shift [simp]:
+  "(+) i ` succs xs 0 = succs xs i"
+  by (force simp: succs_shift [where n=i, symmetric] intro: set_eqI)
+(* Lemma 8.10 *)
+lemma succs_append_otherway [simp]:
+  "succs (xs @ ys) n = succs xs n \<union> succs ys (n + size xs)"
+proof(induction xs arbitrary:n)
+  case Nil
+  then show ?case 
+    by simp
+next
+  case (Cons a xs)
+(* 1. \<And>a xs n. (\<And>n. succs (xs @ ys) n = succs xs n \<union> succs ys (n + size xs)) \<Longrightarrow> succs ((a # xs) @ ys) n = succs (a # xs) n \<union> succs ys (n + size (a # xs))*)
+  then show ?case using algebra_simps sorry
+qed
+
+lemma succs_append [simp]:
+  "succs (xs @ ys) n = succs xs n \<union> succs ys (n + size xs)"
+  apply(induct xs arbitrary: n)
+   apply(auto simp: succs_Cons algebra_simps)
+  done
+
+
+
+theorem ccomp_exec: "ccomp c \<turnstile> (0,s,stk) \<rightarrow>* (size (ccomp c), t, stk) \<Longrightarrow> (c,s) \<Rightarrow> t"
+  sorry
 
 end
